Decidable Eq는 이렇게 구현하는 거구나!

doc/design/DotNet.lean
@@ -16,10 +16,32 @@ instance : Hashable Pos where
   hash p := hash p.val
 
 
+class HasArityDef (α: Type) where
+  arityDef : α → Nat
+
+instance : HasArityDef TypeDef where
+  arityDef td := td.arity
+
+inductive MaybeGeneric (α: Type) [HasArityDef α] where
+  | generic : { a: α // HasArityDef.arityDef a > 0 } → MaybeGeneric α
+  | nonGeneric : { a: α // HasArityDef.arityDef a = 0 } → MaybeGeneric α
+
+def generic? {α: Type} [HasArityDef α] (a: α) : MaybeGeneric α :=
+  let p := HasArityDef.arityDef a > 0
+  Decidable.byCases
+    (fun h1 : p => MaybeGeneric.generic ⟨a, h1⟩)
+    (fun h2 : ¬p => MaybeGeneric.nonGeneric ⟨a, by omega⟩)
+/-
+  if p then
+    MaybeGeneric.generic ⟨a, p⟩
+  else
+    MaybeGeneric.nonGeneric a
+-/
+
 mutual
   inductive TypeCon : Nat → Type 0 where
     | init : (typeDef: TypeDef) → TypeCon typeDef.arity
-    | app : (arity: Pos) → (prev: TypeCon arity) → (typeSpec: TypeSpec) → TypeCon (arity-1)
+    | app : (predArity: Pos) → (pred: TypeCon predArity) → (last: TypeSpec) → TypeCon (predArity-1)
     deriving Hashable
 
   inductive TypeSpec where
@@ -36,8 +58,75 @@ end
 #check TypeCon.noConfusionType
 
 
+def TypeCon.apply {predArity: Pos} (pred: TypeCon predArity) (last: TypeSpec) : TypeCon (predArity-1) :=
+  TypeCon.app predArity pred last
+
+def TypeCon.typeDef (arity: Nat) (typeCon: TypeCon arity) : TypeDef :=
+  match typeCon with
+  | init td => td
+  | app _ typeCon0 _ => typeCon0.typeDef
+
+@[simp]
+theorem TypeCon.typeDef_is_invariant (predArity: Pos) (pred: TypeCon predArity) (last: TypeSpec)
+  : pred.typeDef = (pred.apply last).typeDef := by
+  rfl
+
+def TypeCon.maxLength (arity: Nat) (typeCon: TypeCon arity) : Nat := typeCon.typeDef.arity
+
+abbrev PosTypeCon (arity: Nat) := { tc: TypeCon arity // tc.maxLength > 0 }
+
+
+@[simp]
+theorem TypeCon.maxLength_is_invariant (predArity: Pos) (pred: TypeCon predArity) (last: TypeSpec)
+  : pred.maxLength = (pred.apply last).maxLength := by
+  rfl
+
+def TypeCon.length (arity: Nat) (typeCon: TypeCon arity) : Nat :=
+  match typeCon with
+  | init _ => 0
+  | app _ pred _ => pred.length + 1
+
+@[simp]
+theorem TypeCon.length_init (typeDef: TypeDef) : (TypeCon.init typeDef).length = 0 := by rfl
+
+@[simp]
+theorem TypeCon.length_app (predArity: Pos) (pred: TypeCon predArity) (last: TypeSpec)
+  : pred.length + 1 = (pred.apply last).length := by
+  rfl
+
+def TypeCon.arity_plus_length (arity: Nat) (typeCon: TypeCon arity) : Nat := arity + typeCon.length
+
+namespace Lemma
+namespace ArityPlusLengthIsInvariant
+
+theorem case_of_init_aux (typeDef: TypeDef) (last: TypeSpec) (_: typeDef.arity > 0)
+  : (TypeCon.init typeDef).arity_plus_length = ((TypeCon.init typeDef).apply last).arity_plus_length := by
+  simp
+
+
+end ArityPlusLengthIsInvariant
+end Lemma
+
+--theorem TypeCon.arity_plus_length_is_invariant__case_of_init
+--  (typeDef: TypeDef) (last: TypeSpec)
 
 /-
+theorem TypeCon.arity_plus_length_is_invariant
+  (predArity: Pos) (pred: TypeCon predArity) (last: TypeSpec)
+  : pred.arity_plus_length = (pred.apply last).arity_plus_length := by
+  omega
+
+theorem TypeCon.length_app (predArity: Pos) (pred: TypeCon predArity) (last: TypeSpec)
+  : (TypeCon.app predArity pred last).length = pred.length + 1 := by
+  omega
+
+theorem TypeCon.length_le_maxLength (arity: Nat) (typeCon: TypeCon arity)
+  : typeCon.length <= typeCon.maxLength := by
+  sorry
+
+def TypeCon.typeArgs (typeCon: TypeCon 0) : Vector TypeSpec (typeCon.typeDef.arity) :=
+  sorry
+
 def TypeSpec.eq (ts1 ts2: TypeSpec) : Bool :=
   match (ts1, ts2) with
   | (var, con _) | (con _, var) => .false
